theories/stlc/Symbolic.v
@@ -303,10 +303,6 @@ Qed.
 Module UpDown.
   #[local] Notation "□⇅ A" := (BoxR Acc A) (at level 9, format "□⇅ A", right associativity)
       : indexed_scope.
-  #[local] Notation "□ˢ A" :=
-    (BoxR Sub A)
-      (at level 9, format "□ˢ A", right associativity)
-      : indexed_scope.
   #[local] Notation "w1 .> w2" := (acc_trans w1 w2) (at level 80).
 
   Definition T {A} : ⊢ □⇅A -> A :=
@@ -350,289 +346,6 @@ Module UpDown.
     match r with
       mkAcc _ _ iw pos neg => up_aux pos w2 neg
     end.
-
-  (* Remove phase separation and all abstractions to get
-     a base line. *)
-  Module EagerSolving.
-
-    Import option.notations.
-    Import Unification.
-
-    #[local] Arguments Sub.thin : simpl never.
-
-    Definition M (A : TYPE) : TYPE :=
-      Option (DiamondR Sub A).
-
-    Definition pure {A} : ⊢ A -> M A :=
-      fun w a => Some (existT _ w (Sub.id, a)).
-
-    Definition bind {A B} : ⊢ M A -> □ˢ(A -> (M B)) -> M B :=
-      fun w m f =>
-        '(existT _ w1 (r1,a1)) <- m;;
-        '(existT _ w2 (r2,b2)) <- f w1 r1 a1;;
-        Some (existT _ w2 (r1 ⊙ˢ r2, b2)).
-
-    Fixpoint infer (e : expr) : ⊢ Env -> M Ty :=
-      fun w G =>
-        match e with
-        | v_true => pure w (Ty_bool w)
-        | v_false => pure w (Ty_bool w)
-        | e_if e1 e2 e3 =>
-            '(existT _ w1 (r1 , t1)) <- infer e1 w G;;
-            '(existT _ w2 (r2' , _)) <- mgu t1 (Ty_bool w1);;
-            let r2 := Sub.triangular r2' in
-            let G2 := <{ G ~ r1 ⊙ˢ r2 }> in
-            '(existT _ w3 (r3, t2)) <- infer e2 w2 G2;;
-            let G3 := <{ G2 ~ r3 }> in
-            '(existT _ w4 (r4, t3)) <- infer e3 w3 G3;;
-            '(existT _ w5 (r5' , _)) <- mgu <{ t2 ~ r4 }> t3;;
-            let r5 := Sub.triangular r5' in
-            Some (existT _ w5 (r1 ⊙ˢ (r2 ⊙ˢ (r3 ⊙ˢ (r4 ⊙ˢ r5))), <{ t3 ~ r5 }>))
-        | e_var s => match value s G with
-                     | Some t => pure w t
-                     | None => None
-                     end
-        | e_absu s e =>
-            let w1 := w ▻ 0 in
-            let r1 := Sub.step in
-            let t1 := Ty_hole w1 0 ctx.in_zero in
-            '(existT _ w2 (r2,t2)) <- infer e w1 ((s, t1) :: <{ G ~ r1 }>);;
-            Some (existT _ w2 (r1 ⊙ˢ r2, Ty_func _ <{ t1 ~ r2 }> t2))
-        | e_abst s t e =>
-            let t1 := lift t w in
-            '(existT _ w1 (r1,t2)) <- infer e w ((s, t1) :: G);;
-            Some (existT _ w1 (r1, Ty_func _ <{ t1 ~ r1 }> t2))
-        | e_app e1 e2 =>
-            '(existT _ w1 (r1,t1)) <- infer e1 w G;;
-            let G1 := <{ G ~ r1 }> in
-            '(existT _ w2 (r2,t2)) <- infer e2 w1 G1;;
-            let w3 := w2 ▻ 0 in
-            let r3 := Sub.step in
-            let ti := Ty_hole w3 0 ctx.in_zero in
-            let G3 := <{ G1 ~ r2 ⊙ˢ r3 }> in
-            '(existT _ w4 (r4', _)) <-
-               mgu
-                 <{ t1 ~ r2 ⊙ˢ r3 }>
-                 (Ty_func _ <{ t2 ~ r3 }> ti);;
-            let r4 := Sub.triangular r4' in
-            Some (existT _ w4 (r1 ⊙ˢ (r2 ⊙ˢ (r3 ⊙ˢ r4)), <{ ti ~ r4 }>))
-        end.
-
-    Lemma soundness e :
-      forall (w : World) G,
-        option.wlp
-          (fun '(existT _ w1 (r1, b)) =>
-             forall ι : Assignment w1,
-               exists ee, inst <{ G ~ r1 }> ι |-- e ; inst b ι ~> ee)
-          (infer e w G).
-    Proof.
-      induction e; cbn; intros w G; unfold pure.
-      - constructor; intros ι. exists v_true; cbn. constructor.
-      - constructor; intros ι. exists v_false; cbn. constructor.
-      - rewrite option.wlp_bind.
-        specialize (IHe1 w G). revert IHe1.
-        apply option.wlp_monotonic.
-        intros (w1 & r1 & t1) H1.
-        rewrite option.wlp_bind.
-        destruct (mgu_spec t1 (Ty_bool w1)) as [(w2 & r2 & [])|]; [|constructor].
-        constructor.
-        rewrite option.wlp_bind.
-        specialize (IHe2 w2 (persist w G w2 (r1 ⊙ˢ Sub.triangular r2))).
-        revert IHe2.
-        apply option.wlp_monotonic.
-        intros (w3 & r3 & t2) H2.
-        rewrite option.wlp_bind.
-        specialize (IHe3 w3 (persist w2 (persist w G w2 (r1 ⊙ˢ Sub.triangular r2)) w3 r3)).
-        revert IHe3.
-        apply option.wlp_monotonic.
-        intros (w4 & r4 & t3) H3.
-        rewrite option.wlp_bind.
-        destruct (mgu_spec (persist w3 t2 w4 r4) t3) as [(w5 & r5 & [])|]; [|constructor].
-        constructor. constructor. intros ι.
-        (* Need composition of assignments with Subs. *)
-        admit.
-      - destruct value eqn:?.
-        + constructor. intros. exists (e_var s).
-          constructor.
-          (* need value inst lemma, and persist_subid *)
-          admit.
-        + constructor.
-      - rewrite option.wlp_bind.
-        specialize (IHe (w ▻ 0) (cons (pair s (Ty_hole (ctx.snoc w 0) 0 ctx.in_zero)) (persist w G (ctx.snoc w 0) Sub.step))).
-        revert IHe.
-        apply option.wlp_monotonic.
-        intros (w1 & r1 & t1) H1.
-        constructor.
-        intros ι. specialize (H1 ι). destruct H1 as [e' HT1].
-        cbn. eexists. constructor. cbn in *.
-        (* need persist acc_trans lemma *)
-        admit.
-      - rewrite option.wlp_bind.
-        specialize (IHe w (cons (pair s (lift t w)) G)).
-        revert IHe.
-        apply option.wlp_monotonic.
-        intros (w1 & r1 & t1) H1.
-        constructor.
-        intros ι. specialize (H1 ι). destruct H1 as [e' HT1].
-        cbn. eexists.
-        (* need inst lift lemma *)
-        admit.
-      - rewrite option.wlp_bind.
-        specialize (IHe1 w G).
-        revert IHe1.
-        apply option.wlp_monotonic.
-        intros (w1 & r1 & t1) H1.
-        rewrite option.wlp_bind.
-        specialize (IHe2 w1 (persist _ G _ r1)).
-        revert IHe2.
-        apply option.wlp_monotonic.
-        intros (w2 & r2 & t2) H2.
-        rewrite option.wlp_bind.
-        destruct (mgu_spec
-                    <{ t1 ~ r2 ⊙ˢ Sub.step }>
-                    (Ty_func (w2 ▻ 0) <{ t2 ~ Sub.step }> (Ty_hole (w2 ▻ 0) 0 ctx.in_zero)))
-          as [(w3 & r3 & [])|]; [|constructor].
-        constructor. constructor. intros ι.
-        (* Need composition of assignments with Subs *)
-        admit.
-    Admitted.
-
-    Lemma completeness {G e t ee} (R : G |-- e ; t ~> ee) :
-      forall w : World,
-        option.wp
-          (fun '(existT _ w1 (r1, b)) =>
-             forall w2 (r2 : w1 ⊒ˢ w2),
-             exists w3 (r3 : w2 ⊒ˢ w3), <{ b ~ r2 ⊙ˢ r3 }> = lift t w3)
-          (infer e w (liftEnv G w)).
-    Proof.
-      induction R; cbn - [Sub.step Sub.subst persist]; intros w; unfold pure.
-      - constructor. intros w2 r2. exists w2. exists Sub.id. reflexivity.
-      - constructor. intros w2 r2. exists w2. exists Sub.id. reflexivity.
-
-      - rewrite option.wp_bind.
-        specialize (IHR1 w). revert IHR1.
-        apply option.wp_monotonic.
-        intros (w1 & r1 & t1) H1.
-        rewrite option.wp_bind.
-        destruct (mgu_spec t1 (Ty_bool w1)) as [(w2 & r2 & [])|].
-        2: {
-          exfalso.
-          destruct (H1 w1 Sub.id) as (w2 & r2 & Heq).
-          rewrite Sub.comp_id_left in Heq.
-          eapply (H w2 r2); clear H.
-          apply Heq.
-        }
-        constructor.
-        rewrite option.wp_bind.
-        specialize (IHR2 w2). revert IHR2.
-        rewrite persist_liftEnv.
-        apply option.wp_monotonic.
-        intros (w3 & r3 & t2) H2.
-        rewrite option.wp_bind.
-        specialize (IHR3 w3). revert IHR3.
-        rewrite persist_liftEnv.
-        apply option.wp_monotonic.
-        intros (w4 & r4 & t3) H3.
-        rewrite option.wp_bind.
-        destruct (mgu_spec <{ t2 ~ r4 }> t3) as [(w5 & r5 & [])|].
-        2: {
-          exfalso.
-          specialize (H3 w4 Sub.id). destruct H3 as (w5 & r5 & H3).
-          rewrite Sub.comp_id_left in H3.
-          specialize (H2 w5 (r4 ⊙ˢ r5)). destruct H2 as (w6 & r6 & H2).
-          apply (H0 w6 (r5 ⊙ˢ r6)). clear - H2 H3.
-          cbv [P.max P.unifies persist PersistentSub_Ty] in *.
-          repeat rewrite Sub.subst_comp in *.
-          rewrite H2, H3. rewrite subst_lift. easy.
-        }
-
-        constructor.
-        constructor.
-        intros w6 r6. specialize (H3 w6 (Sub.triangular r5 ⊙ˢ r6)).
-        destruct H3 as (w7 & r7 & H3).
-        exists w7. exists r7. clear - H3.
-        cbv [P.max P.unifies persist PersistentSub_Ty] in *.
-        now repeat rewrite Sub.subst_comp in *.
-
-      - rewrite value_lift. rewrite H.
-        constructor. intros. exists w2. exists Sub.id.
-        now rewrite persist_liftTy.
-
-      - rewrite option.wp_bind.
-        specialize (IHR (w ▻ 0)). revert IHR.
-        rewrite persist_liftEnv. cbn.
-        rename v into x.
-        admit.
-
-      - rewrite option.wp_bind.
-        specialize (IHR w). revert IHR.
-        apply option.wp_monotonic.
-        intros (w1 & r1 & t1) H1.
-        constructor.
-        intros w2 r2.
-        specialize (H1 w2 r2). destruct H1 as (w3 & r3 & H1).
-        exists w3, r3. cbn. f_equal.
-        + now rewrite persist_liftTy, subst_lift.
-        + apply H1.
-
-      - rewrite option.wp_bind.
-        specialize (IHR1 w). revert IHR1.
-        apply option.wp_monotonic.
-        intros (w1 & r1 & tf) H1.
-        rewrite option.wp_bind.
-        specialize (IHR2 w1). revert IHR2.
-        rewrite persist_liftEnv.
-        apply option.wp_monotonic.
-        intros (w2 & r2 & ta) H2.
-        rewrite option.wp_bind.
-        destruct
-          (mgu_spec
-             <{ tf ~ r2 ⊙ˢ Sub.step }>
-             (Ty_func (w2 ▻ 0) <{ ta ~ Sub.step }> (Ty_hole (w2 ▻ 0) 0 ctx.in_zero)))
-          as [(w3 & r3' & [])|].
-        2: {
-          exfalso.
-          specialize (H1 w2 r2).
-          destruct H1 as (w3 & r3 & H1).
-          specialize (H2 w3 r3). destruct H2 as (w4 & r4 & H2).
-          apply (H w4 (Sub.thick ctx.in_zero (lift t1 _) ⊙ˢ r3 ⊙ˢ r4)).
-          cbv [P.max P.unifies persist PersistentSub_Ty Sub.step] in *.
-          cbn - [Sub.thin Sub.thick].
-          repeat rewrite Sub.subst_comp in *.
-          rewrite
-            (Sub.thin_thick_pointful
-              ctx.in_zero
-              (lift t1 w2)
-              (Sub.subst tf r2)).
-          rewrite
-            (Sub.thin_thick_pointful
-              ctx.in_zero
-              (lift t1 w2)
-              ta).
-          cbn. now rewrite H1, H2, ?subst_lift.
-        }
-        constructor.
-        constructor.
-        destruct H as [Hu _].
-        cbv [P.max P.unifies persist PersistentSub_Ty Sub.step] in *.
-        remember (Sub.triangular r3') as r3.
-        clear r3' Heqr3.
-        intros w4 r4.
-        specialize (H1 w4 (r2 ⊙ˢ Sub.thin ctx.in_zero ⊙ˢ r3 ⊙ˢ r4)).
-        destruct H1 as (w5 & r5 & H1).
-        specialize (H2 w5 (Sub.thin ctx.in_zero ⊙ˢ r3 ⊙ˢ r4 ⊙ˢ r5)).
-        destruct H2 as (w6 & r6 & H2).
-        cbn - [Sub.thin Sub.thick] in *.
-        exists w6, (r5 ⊙ˢ r6).
-        rewrite ?Sub.subst_comp in *.
-        rewrite Hu in H1. clear Hu.
-        cbn - [Sub.thin] in H1.
-        injection H1. intros H11 H12. clear H1.
-        now rewrite H11, subst_lift.
-
-    Admitted.
-
-  End EagerSolving.
 
   Definition bind {A B} : ⊢ FreeM A -> □⇅(A -> (FreeM B)) -> FreeM B :=
     fix bind {w} m f :=
@@ -840,3 +553,709 @@ Module UpDown.
   End Attempt3.
 
 End UpDown.
+
+(* Remove phase separation and all abstractions to get
+   a base line. *)
+Module EagerSolving.
+
+  Import option.notations.
+  Import Unification.
+  Import SigTNotations.
+
+  #[local] Arguments Sub.thin : simpl never.
+  #[local] Notation "□ˢ A" :=
+    (BoxR Sub A)
+      (at level 9, format "□ˢ A", right associativity)
+      : indexed_scope.
+
+  Definition T {A} : ⊢ □ˢA -> A :=
+    fun w a => a w Sub.id.
+  Definition K {A B} : ⊢ □ˢ(A -> B) -> □ˢA -> □ˢB :=
+    fun w f a w' r => f _ r (a _ r).
+  Definition _4 {A} : ⊢ □ˢA -> □ˢ□ˢA :=
+    fun w a w1 r1 w2 r2 => a w2 (r1 ⊙ˢ r2).
+
+  Definition M (A : TYPE) : TYPE :=
+    Option (DiamondR Sub A).
+
+  Definition pure {A} : ⊢ A -> M A :=
+    fun w a => Some (existT _ w (Sub.id, a)).
+
+  Definition bind {A B} : ⊢ M A -> □ˢ(A -> (M B)) -> M B :=
+    fun w m f =>
+      '(existT _ w1 (r1,a1)) <- m;;
+      '(existT _ w2 (r2,b2)) <- f w1 r1 a1;;
+      Some (existT _ w2 (r1 ⊙ˢ r2, b2)).
+
+  Definition mexists {A w n} (m : M A (w ▻ n)) : M A w :=
+    '(w';(r,a)) <- m ;;
+    Some (existT _ w' (Sub.step ⊙ˢ r, a)).
+
+  Definition mgu : ⊢ Ty -> Ty -> M Unit :=
+    fun w t1 t2 =>
+      '(w;(r,u)) <- Variant1.mgu t1 t2 ;;
+      Some (w; (Sub.triangular r, u)).
+
+  Fixpoint infer (e : expr) : ⊢ Env -> M Ty.
+  Proof.
+    intros w G. destruct e.
+    - exact (pure w (Ty_bool w)).
+    - exact (pure w (Ty_bool w)).
+    - eapply bind.
+      apply (infer e1 w G).
+      intros w1 r1 t1.
+      eapply bind.
+      apply (mgu w1 t1 (Ty_bool w1)).
+      intros w2 r2 _.
+      eapply bind.
+      apply (infer e2 w2 <{ G ~ r1 ⊙ˢ r2 }>).
+      intros w3 r3 t2.
+      eapply bind.
+      apply (infer e3 w3 <{ G ~ r1 ⊙ˢ r2 ⊙ˢ r3 }>).
+      intros w4 r4 t3.
+      eapply bind.
+      apply (mgu w4 <{ t2 ~ r4 }> t3).
+      intros w5 r5 _.
+      apply pure.
+      exact <{ t3 ~ r5 }>.
+    - destruct (value s G) as [t|].
+      + apply pure. apply t.
+      + apply None.
+    - pose (w ▻ 0) as w1.
+      pose (Ty_hole w1 0 ctx.in_zero) as t1.
+      pose (@Sub.step w 0) as r1.
+      pose ((s, t1) :: <{ G ~ r1 }>) as G1.
+      eapply mexists.
+      eapply bind.
+      apply (infer e w1 G1).
+      intros w2 r2 t2.
+      apply pure.
+      apply (Ty_func _ <{ t1 ~ r2 }> t2).
+    - eapply bind.
+      apply (infer e w ((s,lift t w) :: G)).
+      intros w1 r1 t2.
+      apply pure.
+      apply (Ty_func _ (lift t _) t2).
+    - eapply bind.
+      apply (infer e1 w G).
+      intros w1 r1 t1.
+      pose <{ G ~ r1 }> as G1.
+      eapply bind.
+      apply (infer e2 w1 G1).
+      intros w2 r2 t2.
+      eapply (mexists (n := 0)).
+      pose (w2 ▻ 0) as w3.
+      pose (@Sub.step w2 0) as r3.
+      pose (Ty_hole w3 0 ctx.in_zero) as ti.
+      eapply bind.
+      apply (mgu _ <{ t1 ~ r2 ⊙ˢ r3 }>
+               (Ty_func _ <{ t2 ~ r3 }> ti)).
+      intros w4 r4 _.
+      apply pure.
+      apply <{ ti ~ r4 }>.
+  Defined.
+
+  Definition WLP {A} : ⊢ M A -> □ˢ(A -> PROP) -> PROP :=
+    fun w m P => option.wlp (fun '(w;(r,a)) => P w r a) m.
+
+  Lemma wlp_pure {A w} (a : A w) (p : □ˢ(A -> PROP) w) :
+    WLP w (pure w a) p <-> T w p a.
+  Proof. unfold WLP, pure. now rewrite option.wlp_match. Qed.
+
+  Lemma wlp_bind {A B w} (m : M A w) (k : □ˢ(A -> M B) w) (p : □ˢ(B -> PROP) w) :
+    WLP w (bind _ m k) p <->
+      WLP w m (fun w1 r1 a1 => WLP w1 (k w1 r1 a1) (_4 w p w1 r1)).
+  Proof.
+    unfold WLP, bind.
+    rewrite option.wlp_bind.
+    apply option.wlp_proper.
+    intros (w1 & r1 & a1).
+    rewrite option.wlp_bind.
+    apply option.wlp_proper.
+    intros (w2 & r2 & b2).
+    now rewrite option.wlp_match.
+  Qed.
+
+  Lemma wlp_mexists {A w n} (m : M A (w ▻ n)) (p : □ˢ(A -> PROP) w) :
+    WLP w (mexists m) p <->
+    WLP (w ▻ n) m (_4 w p (w ▻ n) Sub.step).
+  Proof.
+    unfold mexists, WLP, _4.
+    rewrite option.wlp_bind.
+    apply option.wlp_proper.
+    intros (w1 & r1 & a1).
+    now rewrite option.wlp_match.
+  Qed.
+
+  Lemma wlp_monotonic {A w} (m : M A w) :
+    forall
+      (p q : □ˢ(A -> PROP) w)
+      (pq : forall w1 r1 a1, p w1 r1 a1 -> q w1 r1 a1),
+      WLP w m p -> WLP w m q.
+  Proof.
+    intros p q pq. unfold WLP.
+    apply option.wlp_monotonic.
+    intros (w1 & r1 & a1).
+    apply pq.
+  Qed.
+
+  Definition WP {A} : ⊢ M A -> □ˢ(A -> PROP) -> PROP :=
+    fun w m P => option.wp (fun '(w;(r,a)) => P w r a) m.
+
+  Lemma wp_pure {A w} (a : A w) (p : □ˢ(A -> PROP) w) :
+    WP w (pure w a) p <-> T w p a.
+  Proof.
+    unfold WP, pure. now rewrite option.wp_match.
+  Qed.
+
+  Lemma wp_bind {A B w} (m : M A w) (k : □ˢ(A -> M B) w) (p : □ˢ(B -> PROP) w) :
+    WP w (bind _ m k) p <->
+      WP w m (fun w1 r1 a1 => WP w1 (k w1 r1 a1) (_4 w p w1 r1)).
+  Proof.
+    unfold WP, bind.
+    rewrite option.wp_bind.
+    apply option.wp_proper.
+    intros (w1 & r1 & a1).
+    rewrite option.wp_bind.
+    apply option.wp_proper.
+    intros (w2 & r2 & b2).
+    now rewrite option.wp_match.
+  Qed.
+
+  Lemma wp_mexists {A w n} (m : M A (w ▻ n)) (p : □ˢ(A -> PROP) w) :
+    WP w (mexists m) p <->
+    WP (w ▻ n) m (_4 w p (w ▻ n) Sub.step).
+  Proof.
+    unfold mexists, WP, _4.
+    rewrite option.wp_bind.
+    apply option.wp_proper.
+    intros (w1 & r1 & a1).
+    now rewrite option.wp_match.
+  Qed.
+
+  Lemma wp_monotonic {A w} (m : M A w) :
+    forall
+      (p q : □ˢ(A -> PROP) w)
+      (pq : forall w1 r1 a1, p w1 r1 a1 -> q w1 r1 a1),
+      WP w m p -> WP w m q.
+  Proof.
+    intros p q pq. unfold WP.
+    apply option.wp_monotonic.
+    intros (w1 & r1 & a1).
+    apply pq.
+  Qed.
+
+  (* Lemma wlp_mgu {w} (t1 t2 : Ty w) (p : □ˢ(Unit -> PROP) w) : *)
+  (*   (exists w' (r : Sub w w'), *)
+  (*     P.max (P.unifies t1 t2) r /\ p w' r tt) -> *)
+  (*   WLP w (mgu w t1 t2) p. *)
+  (* Proof. *)
+  (*   unfold mgu. unfold WLP. *)
+  (*   rewrite option.wlp_bind. *)
+  (*   rewrite option.wlp_match. *)
+  (*   destruct (mgu_spec t1 t2) as [(w2 & r2 & [])|]. *)
+  (*   - rewrite option.wlp_match. *)
+  (*     split. *)
+  (*     + now exists w2, (Sub.triangular r2). *)
+  (*     + intros (w3 & r3 & H1 & H2). *)
+  (*       admit. *)
+  (* Abort. *)
+
+  Lemma soundness e :
+    forall (w : World) G,
+      WLP w (infer e w G)
+        (fun w1 r1 b =>
+           forall ι : Assignment w1,
+           exists ee, inst <{ G ~ r1 }> ι |-- e ; inst b ι ~> ee).
+  Proof.
+    induction e; cbn - [mexists]; intros w G.
+    - rewrite wlp_pure. intros ι. exists v_true; cbn. constructor.
+    - rewrite wlp_pure. intros ι. exists v_false; cbn. constructor.
+    - rewrite wlp_bind.
+      specialize (IHe1 w G). revert IHe1.
+      apply wlp_monotonic.
+      intros w1 r1 t1 H1.
+      rewrite wlp_bind.
+      unfold WLP at 1, mgu at 2.
+      destruct (mgu_spec t1 (Ty_bool w1)) as [(w2 & r2 & [])|]; [|constructor].
+      constructor.
+      rewrite wlp_bind.
+      specialize (IHe2 w2 (persist w G w2 (r1 ⊙ˢ Sub.triangular r2))).
+      revert IHe2.
+      apply wlp_monotonic.
+      intros w3 r3 t2 H2.
+      rewrite wlp_bind.
+      specialize (IHe3 w3 (persist w G w3 (r1 ⊙ˢ Sub.triangular r2 ⊙ˢ r3))).
+      revert IHe3.
+      apply wlp_monotonic.
+      intros w4 r4 t3 H3.
+      rewrite wlp_bind.
+      unfold WLP at 1, mgu.
+      destruct (mgu_spec (persist w3 t2 w4 r4) t3) as [(w5 & r5 & [])|]; [|constructor].
+      constructor.
+      rewrite wlp_pure.
+      intros ι.
+      (* Need composition of assignments with Subs. *)
+      admit.
+    - destruct value eqn:?.
+      + rewrite wlp_pure. intros ι. exists (e_var s).
+        constructor.
+        (* need value inst lemma, and persist_subid *)
+        admit.
+      + constructor.
+    - rewrite wlp_mexists.
+      rewrite wlp_bind.
+      specialize (IHe (w ▻ 0) (cons (pair s (Ty_hole (ctx.snoc w 0) 0 ctx.in_zero)) (persist w G (ctx.snoc w 0) Sub.step))).
+      revert IHe.
+      apply wlp_monotonic.
+      intros w1 r1 t1 H1.
+      rewrite wlp_pure.
+      intros ι. specialize (H1 ι). destruct H1 as [e' HT1].
+      cbn. eexists. constructor. cbn in *.
+      (* need persist acc_trans lemma *)
+      admit.
+    - rewrite wlp_bind.
+      specialize (IHe w (cons (pair s (lift t w)) G)).
+      revert IHe.
+      apply wlp_monotonic.
+      intros w1 r1 t1 H1.
+      rewrite wlp_pure.
+      intros ι. specialize (H1 ι). destruct H1 as [e' HT1].
+      cbn. eexists.
+      (* need inst lift lemma *)
+      admit.
+    - rewrite wlp_bind.
+      specialize (IHe1 w G).
+      revert IHe1.
+      apply wlp_monotonic.
+      intros w1 r1 t1 H1.
+      rewrite wlp_bind.
+      specialize (IHe2 w1 (persist _ G _ r1)).
+      revert IHe2.
+      apply wlp_monotonic.
+      intros w2 r2 t2 H2.
+      rewrite wlp_mexists.
+      rewrite wlp_bind.
+      unfold WLP at 1, mgu.
+      destruct (mgu_spec
+                  <{ t1 ~ r2 ⊙ˢ Sub.step }>
+                  (Ty_func (w2 ▻ 0) <{ t2 ~ Sub.step }> (Ty_hole (w2 ▻ 0) 0 ctx.in_zero)))
+        as [(w3 & r3 & [])|]; [|constructor].
+      constructor.
+      rewrite wlp_pure.
+      intros ι.
+      (* Need composition of assignments with Subs *)
+      admit.
+  Admitted.
+
+  Definition REL (A : World -> Type) : Type :=
+    forall w0 w1 (r1 : w0 ⊒ˢ w1),
+      A w0 -> A w1 -> Prop.
+
+  Definition RBox {A} (R : REL A) : REL □ˢA :=
+    fun w0 w1 r01 ba0 ba1 =>
+      forall (w2 w3 : World) (r02 : w0 ⊒ˢ w2) (r13 : w1 ⊒ˢ w3) (r23 : w2 ⊒ˢ w3),
+        r01 ⊙ˢ r13 = r02 ⊙ˢ r23 ->
+        R w2 w3 r23 (ba0 w2 r02) (ba1 w3 r13).
+
+   (*         r01 *)
+   (*    w0 -------> w1 *)
+   (*     |          | *)
+   (* r02 |          | r13 *)
+   (*     |    //    | *)
+   (*     ↓          ↓ *)
+   (*    w2 -------> w3 *)
+   (*         r23 *)
+
+  Definition RDSub {A} (R : REL A) : REL <[Sub]>A.
+  Proof.
+    intros w0 w1 r01.
+    intros (w2 & r02 & a2).
+    intros (w3 & r13 & a3).
+    refine (exists r23,
+               r01 ⊙ˢ r13 = r02 ⊙ˢ r23 /\ R _ _ r23 a2 a3).
+  Defined.
+
+  Definition RImpl {A B} (RA : REL A) (RB : REL B) : REL (Impl A B) :=
+    fun w0 w1 r01 f0 f1 =>
+      forall a0 a1,
+        RA w0 w1 r01 a0 a1 ->
+        RB w0 w1 r01 (f0 a0) (f1 a1).
+
+  Definition ROption {A} (R : REL A) : REL (Option A) :=
+    fun w0 w1 r01 m0 m1 =>
+      match m0 , m1 with
+      | Some a0 , Some a1 => R w0 w1 r01 a0 a1
+      | Some _  , None    => True
+      | None    , Some _  => False
+      | None    , None    => True
+      end.
+
+  Definition RTy : REL Ty :=
+    fun w0 w1 r01 t0 t1 =>
+      t1 = Sub.subst t0 r01.
+
+  Lemma rty_bool {w0 w1 r01} :
+    RTy w0 w1 r01 (Ty_bool _) (Ty_bool _).
+  Proof.
+    reflexivity.
+  Qed.
+
+  Lemma rty_func {w0 w1 r01} t1_0 t1_1 t2_0 t2_1 :
+    RTy w0 w1 r01 t1_0 t1_1 ->
+    RTy w0 w1 r01 t2_0 t2_1 ->
+    RTy w0 w1 r01 (Ty_func _ t1_0 t2_0) (Ty_func _ t1_1 t2_1).
+  Proof. unfold RTy; cbn; intros; now f_equal. Qed.
+
+  Definition REnv : REL Env.
+  Admitted.
+
+  Definition RM {A} (R : REL A) : REL (M A) :=
+    ROption (RDSub R).
+
+  Definition RValid {A} (R : REL A) (a : ⊢ A) : Prop :=
+    forall w0 w1 r01,
+      R w0 w1 r01 (a w0) (a w1).
+
+  Definition RUnit : REL Unit :=
+    fun _ _ _ _ _ => True.
+
+  Lemma rsome {A} (R : REL A) w0 w1 (r01 : Sub w0 w1) (a0 : A w0) (a1 : A w1) (ra : R w0 w1 r01 a0 a1) :
+    ROption R w0 w1 r01 (Some a0) (Some a1).
+  Proof. apply ra. Qed.
+
+  Lemma rpure {A} (R : REL A) :
+    RValid (RImpl R (RM R)) pure.
+  Proof.
+    intros w0 w1 r01 a0 a1 ra.
+    refine (@rsome _ (RDSub R) w0 w1 r01 _ _ _).
+    unfold RDSub. exists r01. split; auto.
+    now rewrite Sub.comp_id_left, Sub.comp_id_right.
+  Qed.
+
+  Lemma rbind {A B} (RA : REL A) (RB : REL B) :
+    RValid (RImpl (RM RA) (RImpl (RBox (RImpl RA (RM RB))) (RM RB))) bind.
+  Proof.
+    unfold RValid, RImpl, RBox, RM.
+    intros w0 w1 r01.
+    intros [(w2 & r2 & a2)|] [(w3 & r3 & a3)|] rm f0 f1 rf; cbn in rm.
+    - destruct rm as (r23 & Heqr & ra).
+      specialize (rf _ _ r2 r3 r23 Heqr _ _ ra).
+      cbn. revert rf.
+      destruct f0 as [(w4 & r4 & b4)|], f1 as [(w5 & r5 & b5)|]; cbn.
+      + intros (r45 & Heqr2 & rb).
+        exists r45.
+        rewrite <- ?Sub.comp_assoc.
+        rewrite Heqr.
+        rewrite ?Sub.comp_assoc.
+        now rewrite Heqr2.
+      + auto.
+      + auto.
+      + auto.
+    - cbn. destruct f0 as [(w4 & r4 & b4)|]; cbn.
+      + auto.
+      + auto.
+    - cbn. destruct f1 as [(w5 & r5 & b5)|]; cbn.
+      + auto.
+      + auto.
+    - cbn.
+      auto.
+  Qed.
+
+  Lemma rmgu :
+    RValid (RImpl RTy (RImpl RTy (RM RUnit))) mgu.
+  Proof.
+    unfold RValid, RImpl, RM, RUnit.
+    intros w0 w1 r01 t1_0 t1_1 rt1 t2_0 t2_1 rt2.
+    unfold mgu.
+    destruct (mgu_spec t1_0 t2_0) as [(w2 & r02 & ?)|],
+        (mgu_spec t1_1 t2_1) as [(w3 & r13 & ?)|]; cbn.
+    - unfold RTy in *.
+      clear u u0.
+      subst.
+      destruct H0 as [H0 _].
+      destruct H as [_ H].
+      unfold P.unifies in *.
+      specialize (H _ (r01 ⊙ˢ Sub.triangular r13)).
+      rewrite ?Sub.subst_comp in H.
+      specialize (H H0).
+      destruct H as (r23 & ?).
+      exists r23. split; auto.
+    - auto.
+    - apply (H w3 (r01 ⊙ˢ Sub.triangular r13)).
+      destruct H0 as [H0 _].
+      unfold RTy in *.
+      subst. unfold P.unifies in *.
+      now rewrite ?Sub.subst_comp, H0.
+    - auto.
+  Qed.
+
+  Definition rexists {A} (R : REL A) w0 w1 (r01 : Sub w0 w1) {n} (m0 : M A (w0 ▻ n)) (m1 : M A (w1 ▻ n)) :
+    RM R (w0 ▻ n) (w1 ▻ n) (Sub.up1 r01) m0 m1 ->
+    RM R w0 w1 r01 (mexists m0) (mexists m1).
+  Proof.
+    unfold RM, ROption, mexists.
+    destruct m0 as [(w2 & r02 & a2)|], m1 as [(w3 & r13 & a3)|]; cbn - [Sub.step Sub.up1]; auto.
+    intros (r23 & Heqr & ra).
+    exists r23. split; auto.
+    rewrite Sub.comp_assoc, <- Heqr.
+    clear.
+    rewrite <- ?Sub.comp_assoc. f_equal.
+    admit.
+  Admitted.
+
+  Arguments mexists : simpl never.
+
+  Lemma infer_mon (e : expr) :
+    RValid (RImpl REnv (RM RTy)) (infer e).
+  Proof.
+    induction e; cbn [infer]; intros w0 w1 r01 G0 G1 HG.
+    - apply rpure. apply rty_bool.
+    - apply rpure. apply rty_bool.
+
+    - eapply rbind. now apply IHe1.
+      intros w2 w3 r02 r13 r23 Heqr23 t1_2 t1_3 rt1.
+      eapply rbind. apply rmgu; auto. apply rty_bool.
+      intros w4 w5 r24 r35 r45 Heqr45 _ _ _.
+      eapply rbind. apply IHe2. admit.
+      intros w6 w7 r46 r57 r67 Heqr67 t2_6 t2_7 rt2.
+      eapply rbind. apply IHe3. admit.
+      intros w8 w9 r68 r89 r79 Heqr79 t3_8 t3_9 rt3.
+      eapply rbind. apply rmgu; auto.
+      { unfold RTy in *. subst.
+        unfold persist, PersistentSub_Ty.
+        now rewrite <- ?Sub.subst_comp, Heqr79.
+      }
+      intros ? ? ? ? ? ? _ _ _.
+      apply rpure.
+      { unfold RTy in *. subst.
+        unfold persist, PersistentSub_Ty.
+        now rewrite <- ?Sub.subst_comp, H.
+      }
+
+    - admit.
+
+    - apply rexists.
+      eapply rbind. apply IHe. admit.
+      intros w2 w3 r02 r13 r23 Heqr23 t1_2 t1_3 rt1.
+      apply rpure.
+      apply rty_func; auto.
+      { unfold RTy in *. subst.
+        unfold persist, PersistentSub_Ty.
+        now rewrite <- Sub.subst_comp, <- Heqr23.
+      }
+
+    - eapply rbind. apply IHe. admit.
+      intros w2 w3 r02 r13 r23 Heqr23 t1_2 t1_3 rt1.
+      apply rpure.
+      apply rty_func; auto.
+      { unfold RTy. now rewrite subst_lift. }
+
+    - eapply rbind. apply IHe1; auto.
+      intros w2 w3 r02 r13 r23 Heqr23 t1_2 t1_3 rt1.
+      eapply rbind. apply IHe2; auto. admit.
+      intros w4 w5 r24 r35 r45 Heqr45 t2_4 t2_5 rt2.
+      apply rexists.
+      eapply rbind. apply rmgu.
+      { unfold RTy in *. subst.
+        unfold persist, PersistentSub_Ty.
+        rewrite <- ?Sub.subst_comp. f_equal.
+        rewrite <- Sub.comp_assoc.
+        rewrite Heqr45.
+        rewrite ?Sub.comp_assoc. f_equal.
+        admit.
+      }
+      { unfold RTy in *. subst.
+        unfold persist, PersistentSub_Ty.
+        cbn - [Sub.step].
+        rewrite <- ?Sub.subst_comp.
+        f_equal.
+        f_equal.
+        admit.
+      }
+      intros w6 w7 r46 r57 r67 Heqr6 _ _ _.
+      apply rpure.
+      { unfold RTy in *. subst.
+        unfold persist, PersistentSub_Ty.
+        rewrite <- ?Sub.subst_comp.
+        now rewrite <- Heqr6.
+      }
+  Admitted.
+
+  Definition RPropImpl : REL PROP :=
+    fun w0 w1 r01 p q => (q -> p)%type.
+
+  Lemma wp_monotonic_strong {A} (R : REL A) :
+    RValid (RImpl (RM R) (RImpl (RBox (RImpl R RPropImpl)) RPropImpl)) WP.
+  Proof.
+    intros w0 w1 r01 m0 m1 rm p0 p1 rp.
+    unfold RBox, RImpl, RPropImpl in *.
+    unfold RM, ROption, RDSub in rm.
+    destruct m0 as [(w2 & r02 & a2)|], m1 as [(w3 & r13 & a3)|].
+    - unfold RM, ROption, RDSub in rm.
+      destruct rm as (r23 & Heqr & ra).
+      unfold WP. rewrite option.wp_match.
+      intros Hp1. constructor. revert Hp1.
+      eapply rp; eauto.
+    - inversion 1.
+    - destruct rm.
+    - inversion 1.
+  Qed.
+
+  Lemma completeness {G e t ee} (R : G |-- e ; t ~> ee) :
+    forall w : World,
+      WP w (infer e w (liftEnv G w))
+        (fun w1 r1 T =>
+           forall w2 (r2 : w1 ⊒ˢ w2),
+           exists w3 (r3 : w2 ⊒ˢ w3), <{ T ~ r2 ⊙ˢ r3 }> = lift t w3).
+  Proof.
+    Set Printing Depth 18.
+    induction R; cbn - [Sub.step Sub.subst persist]; intros w.
+    - rewrite wp_pure. intros w2 r2. exists w2. exists Sub.id. reflexivity.
+    - rewrite wp_pure. intros w2 r2. exists w2. exists Sub.id. reflexivity.
+
+    - rewrite wp_bind.
+      specialize (IHR1 w). revert IHR1.
+      apply wp_monotonic. intros w1 r1 t1 H1.
+      rewrite wp_bind.
+      unfold mgu at 1, WP at 1.
+      rewrite option.wp_bind.
+      destruct (mgu_spec t1 (Ty_bool w1)) as [(w2 & r2 & [])|].
+      2: {
+        exfalso.
+        destruct (H1 w1 Sub.id) as (w2 & r2 & Heq).
+        rewrite Sub.comp_id_left in Heq.
+        eapply (H w2 r2); clear H.
+        apply Heq.
+      }
+      constructor.
+      constructor.
+      rewrite wp_bind.
+      specialize (IHR2 w2). revert IHR2.
+      rewrite persist_liftEnv.
+      apply wp_monotonic.
+      intros w3 r3 t2 H2.
+      rewrite wp_bind.
+      specialize (IHR3 w3). revert IHR3.
+      rewrite persist_liftEnv.
+      apply wp_monotonic.
+      intros w4 r4 t3 H3.
+      rewrite wp_bind.
+      unfold mgu at 1, WP at 1.
+      rewrite option.wp_bind.
+      destruct (mgu_spec <{ t2 ~ r4 }> t3) as [(w5 & r5 & [])|].
+      2: {
+        exfalso.
+        specialize (H3 w4 Sub.id). destruct H3 as (w5 & r5 & H3).
+        rewrite Sub.comp_id_left in H3.
+        specialize (H2 w5 (r4 ⊙ˢ r5)). destruct H2 as (w6 & r6 & H2).
+        apply (H0 w6 (r5 ⊙ˢ r6)). clear - H2 H3.
+        cbv [P.max P.unifies persist PersistentSub_Ty] in *.
+        repeat rewrite Sub.subst_comp in *.
+        rewrite H2, H3. rewrite subst_lift. easy.
+      }
+
+      constructor.
+      constructor.
+      rewrite wp_pure.
+      unfold T, _4.
+      intros w6 r6. specialize (H3 w6 (Sub.triangular r5 ⊙ˢ r6)).
+      destruct H3 as (w7 & r7 & H3).
+      exists w7. exists r7. clear - H3.
+      cbv [P.max P.unifies persist PersistentSub_Ty] in *.
+      now repeat rewrite Sub.subst_comp in *.
+
+    - rewrite value_lift. rewrite H. cbn.
+      rewrite wp_pure. intros w1 r1.
+      exists w1. exists Sub.id.
+      now rewrite persist_liftTy.
+
+    - rewrite wp_mexists.
+      rewrite wp_bind.
+      specialize (IHR w). revert IHR.
+      rewrite persist_liftEnv.
+      cbn - [Sub.subst].
+      apply (wp_monotonic_strong RTy (w ▻ 0) w (Sub.thick ctx.in_zero (lift vt _))).
+      cbn - [Sub.thick].
+      apply infer_mon. admit.
+      intros w2 w3 r02 r13 r23 Heq t_2 t_3 rt IH.
+      cbn - [Sub.thick] in Heq.
+      rewrite wp_pure.
+      unfold RTy in *. subst.
+      unfold T, _4, persist,  PersistentSub_Ty in *.
+      remember (Ty_hole (w ▻ 0) 0 ctx.in_zero) as tfresh.
+      admit.
+
+    - rewrite wp_bind.
+      specialize (IHR w). revert IHR.
+      apply wp_monotonic.
+      intros w1 r1 t1 H1.
+      rewrite wp_pure.
+      intros w2 r2.
+      specialize (H1 w2 r2). destruct H1 as (w3 & r3 & H1).
+      exists w3, r3. cbn. f_equal.
+      + now rewrite subst_lift.
+      + apply H1.
+
+    - rewrite wp_bind.
+      specialize (IHR1 w). revert IHR1.
+      apply wp_monotonic.
+      intros w1 r1 tf H1.
+      rewrite wp_bind.
+      specialize (IHR2 w1). revert IHR2.
+      rewrite persist_liftEnv.
+      apply wp_monotonic.
+      intros w2 r2 ta H2.
+      rewrite wp_mexists.
+      rewrite wp_bind.
+      unfold mgu, WP at 1.
+      rewrite option.wp_bind.
+      destruct
+        (mgu_spec
+         <{ tf ~ r2 ⊙ˢ Sub.step }>
+           (Ty_func (w2 ▻ 0) <{ ta ~ Sub.step }> (Ty_hole (w2 ▻ 0) 0 ctx.in_zero)))
+        as [(w3 & r3' & [])|].
+      2: {
+        exfalso.
+        specialize (H1 w2 r2).
+        destruct H1 as (w3 & r3 & H1).
+        specialize (H2 w3 r3). destruct H2 as (w4 & r4 & H2).
+        apply (H w4 (Sub.thick ctx.in_zero (lift t1 _) ⊙ˢ r3 ⊙ˢ r4)).
+        cbv [P.max P.unifies persist PersistentSub_Ty Sub.step] in *.
+        cbn - [Sub.thin Sub.thick].
+        repeat rewrite Sub.subst_comp in *.
+        rewrite
+          (Sub.thin_thick_pointful
+             ctx.in_zero
+             (lift t1 w2)
+             (Sub.subst tf r2)).
+        rewrite
+          (Sub.thin_thick_pointful
+             ctx.in_zero
+             (lift t1 w2)
+             ta).
+        cbn. now rewrite H1, H2, ?subst_lift.
+      }
+      constructor.
+      constructor.
+      rewrite wp_pure.
+      destruct H as [Hu _].
+      cbv [P.max P.unifies persist PersistentSub_Ty Sub.step] in *.
+      remember (Sub.triangular r3') as r3.
+      clear r3' Heqr3.
+      intros w4 r4.
+      specialize (H1 w4 (r2 ⊙ˢ Sub.thin ctx.in_zero ⊙ˢ r3 ⊙ˢ r4)).
+      destruct H1 as (w5 & r5 & H1).
+      specialize (H2 w5 (Sub.thin ctx.in_zero ⊙ˢ r3 ⊙ˢ r4 ⊙ˢ r5)).
+      destruct H2 as (w6 & r6 & H2).
+      cbn - [Sub.thin Sub.thick] in *.
+      exists w6, (r5 ⊙ˢ r6).
+      rewrite ?Sub.subst_comp in *.
+      rewrite Hu in H1. clear Hu.
+      cbn - [Sub.thin] in H1.
+      injection H1. intros H11 H12. clear H1.
+      now rewrite H11, subst_lift.
+
+  Admitted.
+
+End EagerSolving.
